Refactoring Splits/LoopSplits

Disjoint.v
@@ -73,254 +73,60 @@ Module Disjoint.
     -> In (fst s') (map fst (loop_splits s)).
   Admitted.
   
+  Lemma disjoint_map_fst {A B : Type} (l1 l2 : list (A*B)) (l1' l2' : list A) :
+    l1' = map fst l1
+    -> l2' = map fst l2
+    -> Disjoint l1' l2'
+    -> Disjoint l1 l2.
+  Admitted.
+
+  Definition innermost_loop p qh :=
+    in_loop p qh /\ forall qh', in_loop p qh -> in_loop qh qh'.
   
-  Definition DivergenceWitness (br : Lab) x xb t t' := 
-    (exists (l : Tag) u u', val_true (u x) =/= val_true (u' x) /\
-                    In (br, l, u) t /\
-                    In (br, l, u') t' /\
-                    exists tt ff, branch br = Some (tt, ff, x, xb)).
+  Lemma tag_eq_ex_innermost_lh q q' j l p i :
+    TPath' ((q',j) :<: nl_rcons l (q,j))
+    -> In (p,i) l
+    -> i = j \/ exists lh, innermost_loop p lh /\ In lh (map fst l).
+  Admitted.
 
-(*  Lemma different_tgt_is_branch {br : Lab} {i : Tag} {s s' : State} {k k' : Conf} :
-    eff (br, i, s) = Some k ->
-    eff (br, i, s') = Some k' ->
-    lab_of k =/= lab_of k' ->
-    exists x, val_true (s x) =/= val_true (s' x) /\ is_branch br x.
-  Proof.
-    intros Hstep Hstep' Hneq.
-    assert (Hspec := branch_spec br).
-    destruct (branch br) as [ [[[tt ff] x] xb] | ] eqn:Hbr.
-    + destruct Hspec as [Hneqtf Hspec].
-      assert (Hspec' := Hspec i s' k' Hstep').
-      specialize (Hspec i s k Hstep).
-      destruct k as [[q j] r], k' as [[q' j'] r']. simpl in *.
-      exists x. split.
-      - destruct (val_true (s x)) eqn:Hv, (val_true (s' x)) eqn:Hv';
-          subst; firstorder.
-      - unfold is_branch. firstorder.
-    + specialize (Hspec i i s s' k k' Hstep Hstep'). firstorder.
-  Qed.*)
-
-(*  Lemma single_edge_disjoint_path (q a q' : Lab) x (p : Path a q') :
-    is_branch a x ->
-    ~ PathIn q p ->
-    a --> q -
-> 
-    exists p', DisjointBranch a x q' q p p'.
-  Proof.
-    intros Hbr Hnin Hedge.
-    exists (PathStep a a q (PathInit a) Hedge).
-    unfold DisjointBranch.
-    split. assumption.
-    intros p' H H'.
-    simpl in H'.
-    inversion_clear H'.
-    rewrite H0 in *. clear H0. contradiction H. eauto.
-  Qed.
-
-  Lemma single_edge_disjoint_path_detail (q a q' : Lab) l u j r x
-        (step : eff (a, l, u) = Some (q, j, r)) (p : Path a q') :
-    is_branch a x ->
-    ~ PathIn q p ->
-    DisjointBranch a x q' q p (step_exists_path step).
-  Proof.
-    simpl.
-    intros Hbr Hnin.
-    unfold DisjointBranch.
-    split; try assumption.
-    intros p' H H'.
-    simpl in H'.
-    inversion_clear H'; [| eauto].
-    rewrite H0 in *. contradiction H. 
-  Qed.
-
-  Lemma contains_label_tag_disjoint p q q' i j j' s s' r r' t t' : 
-    label_tag_in_trace q j (q', j', r') t' = true ->
-    eff (q, j, r) = Some (p, i, s) ->
-    eff (q', j', r') = Some (p, i, s') ->
-    q =/= q' \/ j =/= j' ->
-    exists x xb, (exists a b, DisjointBranch q x q q' a b) /\
-            DivergenceWitness q x xb (q, j, r) (q', j', r') t t'.
-  Proof.
-    intros Hintr Hstep Hstep' Hneq.
-    apply label_tag_in_trace_in in Hintr.
-    destruct Hintr as [u Hinq].
-    + assert (Hnext := Hinq).
-      apply in_succ_exists in Hnext.
-      destruct Hnext as [[k' [Hnext Hin]] | H]; [| injection H; intros; subst; firstorder ].
-      destruct k' as [[b m] w].
-      enough (b =/= p).
-      * specialize (different_tgt_is_branch Hnext Hstep H) as Hbr.
-        destruct Hbr as [x [Hneqx Hbr]].
-        unfold is_branch in Hbr.
-        destruct Hbr as [tt [ff [xb Hbr]]]. exists x, xb.
-        split; simpl.
-        - unfold DisjointBranch.
-          exists (PathInit q). eexists (proj1_sig (path_for_trace _ _ _ Hinq)).
-          split; [ firstorder |].
-          intros p' Paq' Paa. simpl in Paa. eauto.
-        - exists j, r, u. symmetry in Hneqx. unfold is_branch in Hbr.
-          repeat split; try eauto; try constructor.
-      * intro. rewrite H in *. clear H. eapply ivec_fresh.
-        apply Hstep'. apply Hin. eauto using ivec_det.
-  Qed.
-
-  Lemma last_instance p q q' i j j' s' r' t' :
-    eff (q', j', r') = Some (p, i, s') -> 
-    label_tag_in_trace q j (q', j', r') t' = false ->
-    forall j'', last_inst_of q (q', j', r') t' = Some j'' ->
-                j <> j''.
-  Proof.
-    intros Hstep' Hqq' j'' Hinst.
-    eapply not_label_tag_in_trace_in in Hqq'. intro. subst j''. eapply Hqq'.
-    eauto using last_inst_in.
-  Qed.
-
-  Lemma not_contains_label_tag_last_common p q q' i j j' s' r r' t t' :
-    eff (q', j', r') = Some (p, i, s') -> 
-    label_tag_in_trace q j (q', j', r') t' = false ->
-    label_tag_in_trace q' j' (q, j, r) t = false ->
-    (exists br x xb, (exists m w Hinbr Pbrq, 
-                      let Pbrq' := proj1_sig (path_for_trace (q', j', r') t' (br, m, w) Hinbr) in
-                      DisjointBranch br x q' q Pbrq' Pbrq) /\
-                  (exists m w, In (q, j, r) t (br, m, w)) /\ 
-                  (last_inst_of br (q', j', r') t' = last_inst_of br (q, j, r) t ->
-                   DivergenceWitness br x xb (q', j', r') (q, j, r) t' t)) \/
-    (exists j'', j <> j'' /\ last_inst_of q (q', j', r') t' = Some j'') \/
-    (exists j'', j' <> j'' /\ last_inst_of q' (q, j, r) t = Some j'').
-  Proof.
-    intros Hstep' Hqq' Hq'q.
-    dependent induction t.
-    - apply not_label_tag_in_trace_in in Hqq'.
-      exfalso. apply Hqq'.
-      clear Hqq' Hq'q Hstep'.
-      induction t'.
-      + exists s; eauto using In. 
-      + destruct IHt'; eauto using In.
-    - destruct k' as [[a l] u].
-      simpl in Hq'q. conv_bool. destruct Hq'q as [Hnj Hnq].
-      destruct (label_tag_in_trace a l (q', j', r') t') eqn:Hal.
-      + clear IHt.
-
-        (* show that q',j' cannot be the branch *)
-        apply not_label_tag_in_trace_in in Hnq.
-        assert (Haq: (a, l) =/= (q', j')). {
-          intro. apply Hnq. injection H; intros; subst. exists u. constructor.
-        }
-        
-        (* show that a,l has a successor that is on the q',j' trace *)
-        apply label_tag_in_trace_in in Hal. destruct Hal as [u' Hain].
-        assert (Hain' := Hain).
-        eapply in_succ_exists in Hain'.
-        inversion_clear Hain'.
-        -- destruct H as [[[b m] w] [step Hxin]].
-           enough (q =/= b).
-           ++ destruct (last_inst_of q (q', j', r') t') as [j''|] eqn:Hinst;
-                [ right; eauto using last_instance |].
-              assert (Hdiff := different_tgt_is_branch e step H).
-              destruct Hdiff as [x [Hneqx Hbr]]. unfold is_branch in Hbr.
-              destruct Hbr as [tt [ff [xb Hbr]]].
-              left. eapply last_inst_not_exists in Hinst. exists a, x, xb. split.
-              ** exists l, u', Hain.
-                 eapply (not_in_trace_exists_path _ _ _ _ Hain) in Hinst. 
-                 assert (Hbr' : is_branch a x) by (firstorder).
-                 eauto 30 using single_edge_disjoint_path, step_conf_implies_edge. 
-              ** split.
-                 --- exists l, u. eauto using In.
-                 --- unfold DivergenceWitness.
-                     simpl in Hbr. exists l, u', u. symmetry in Hneqx.
-                     repeat split; eauto; try repeat constructor.
-           ++ intro. rewrite H in *. clear H.
-              replace m with j in * by (eauto using ivec_det).
-              apply not_label_tag_in_trace_in in Hqq'. apply Hqq'; eauto.
-        -- injection H; intros; subst. exfalso. apply Hnq. exists u. constructor.
-      + destruct (last_inst_of q (q', j', r') t') as [l''|] eqn:Hinst;
-          [ right; eauto using last_instance |].
-        eapply last_inst_not_exists in Hinst.
-        edestruct IHt; eauto; clear IHt.
-        * left. destruct H as [br [x [xb [Hdisj [Hinbr' Hwit]]]]].
-          exists br, x, xb. split.
-          ** clear Hwit.
-             destruct Hdisj as [m [w [Hinbr [Pbra [Hbr Hdisj]]]]].
-             exists m, w, Hinbr. eapply step_conf_implies_edge in e.
-             eexists (PathStep br a q Pbra e).
-             split; [ eassumption |].
-             intros p'. intros Pbrq'1. intros Pbrq1. eapply Hdisj; eauto.
-             destruct Pbrq1; try eassumption.
-             exfalso. rewrite H in *. clear H.
-             eapply (not_in_trace_exists_path _ _ _ _ Hinbr) in Hinst. simpl in *. eauto.
-          ** split.
-             *** destruct Hinbr' as [l' [u' Hinbr']].
-                 exists l', u'. eauto using In.
-             *** clear Hdisj. intros Hlast.
-                 simpl in Hlast.
-                 destruct (br == q).
-                 ++ rewrite <- e0 in *. clear e0. conv_bool.
-                    exfalso. eapply not_label_tag_in_trace_in. eapply Hqq'. eapply last_inst_in.
-                    eassumption.
-                 ++ replace (br ==b q) with false in Hlast
-                     by (symmetry; apply beq_false; eassumption).
-                    specialize (Hwit Hlast). clear Hlast.
-                    destruct Hwit as [m [w [w' [Hneq [Hin [Hin' Hbr]]]]]].
-                    unfold DivergenceWitness.
-                    exists m, w, w'.
-                    repeat split; try repeat constructor; eauto.
-        * destruct H as [[l' [Hlneq Hlast]] | [j'' [Hjneq Hlast]]].
-          eapply last_inst_in in Hlast. destruct Hlast as [u' Hlast].
-          destruct (branch a) as [[[[tt ff] x] xb] | ] eqn:Hbr.
-          ++ left. exists a, x, xb. split.
-             ** exists l', u', Hlast.
-                eapply (not_in_trace_exists_path _ _ _ _ Hlast) in Hinst. simpl in *.
-                assert (Hbr': is_branch a x) by (unfold is_branch; eauto).
-                eauto using single_edge_disjoint_path, step_conf_implies_edge.
-             ** split.
-                *** exists l, u. eauto using In.
-                *** intros. unfold DivergenceWitness. simpl in H.
-                    exfalso. 
-                    destruct (a == q).
-                    -- rewrite <- e0 in *. clear e0.
-                       eapply not_label_tag_in_trace_in. eapply Hqq'. 
-                       eauto using last_inst_in. 
-                    -- rewrite last_inst_self in H.
-                       eapply not_label_tag_in_trace_in. eapply Hal. eauto using last_inst_in.
-          ++ assert (Hbrspec := branch_spec a). rewrite Hbr in Hbrspec.
-             eapply in_succ_exists in Hlast.
-             inversion_clear Hlast.
-             ** destruct H as [[[b m] w] [Hnext' Hin']].
-                specialize (Hbrspec l l' u u' _ _ e Hnext').
-                simpl in Hbrspec. subst b. exfalso. apply Hinst.
-                exists m, w; assumption.
-             ** injection H; intros; subst; clear H.
-                specialize (Hbrspec l l' _ _ _ _ e Hstep'). simpl in Hbrspec. subst q.
-                right. right. exists l. split; [ firstorder |]. eapply last_inst_step_pred.
-                intro. apply Hinst. rewrite <- H in *. exists l', u'. constructor.
-          ++ right. right. exists j''. split; [ firstorder |]. simpl.
-             destruct (q' == q); try eassumption.
-             rewrite <- e0 in *. exfalso. apply Hinst. exists j', r'. constructor.
-  Qed.
-
-  Lemma disjoint_contains p q q' i j j' s s' r r' t t' :
-    label_tag_in_trace q j (q', j', r') t' = true ->
-    eff (q, j, r) = Some (p, i, s) ->
-    eff (q', j', r') = Some (p, i, s') ->
-    q =/= q' ->
-    exists br x xb, DivergenceWitness br x xb (q, j, r) (q', j', r') t t' /\ List.In (br, x) (splits p).
-                 
-  Proof.
-    intros Hcont Hstep Hstep' Hneq.
-    edestruct contains_label_tag_disjoint as [x [xb [Hdis Hwit]]]; eauto.
-    destruct Hdis as [a [b [Hbr Hdis]]].
-    exists q, x, xb. split; eauto.
-    eapply splits_spec. 
-    exists q, q'. eexists. eexists.
-    repeat split; eauto using step_conf_implies_edge.
-  Qed.
-
-  Lemma witness_commutative br x xb q q' j j' r r' t t' :
-    DivergenceWitness br x xb (q, j, r) (q', j', r') t t' <->
-    DivergenceWitness br x xb (q', j', r') (q, j, r) t' t.
-  Proof.
-    unfold DivergenceWitness.
-    split; intros; destruct H as [l [u [u' [Hneq [Hin [Hin' Hbr]]]]]]; exists l, u', u; firstorder.
-  Qed.*)
+  
+  Hint Unfold CPath.
     
+  Lemma disj_loopheads p i q l1 l2 qh :
+    TPath' ((p,i) :<: nl_rcons l1 (q,i))
+    -> TPath' ((p,i) :<: nl_rcons l2 (q,i))
+    -> Disjoint l1 l2
+    -> loop_head qh
+    -> In qh (map fst l1)
+    -> ~ In qh (map fst l2).
+  Admitted.
+
+  (* This is wrong! This holds only for the FIRST header.
+  Lemma loop_head_tag_cases l q i qh j :
+    TPath' (nl_rcons l (q,i))
+    -> loop_head qh
+    -> In (qh,j) l
+    -> j = O :: i
+      \/ match i with
+        | nil => False
+        | m :: i' => j = S m :: i'
+        end.
+  Admitted.
+  *)
+
+  Lemma lab_tag_same_length c0 c c' p i j l l' :
+    TPath c0 c l (* the paths need to have the same origin *)
+    -> TPath c0 c' l'
+    -> (p,i) ∈ l
+    -> (p,j) ∈ l'
+    -> length i = length j.
+  Admitted.
+
+  Lemma tag_length_inbetween p i l q q' j :
+    TPath' ((p,i) :<: nl_rcons l (q,i))
+    -> (q',j) ∈ l
+    -> length i <= length j.
+    (* because if we would exit a loop, we could never achieve to get the same tag again *)
+  Admitted.
+  
 End Disjoint.
