LoopSplits.v
@@ -1,0 +1,29 @@
+Require Import Coq.Classes.EquivDec.
+Require Import Coq.Classes.RelationClasses.
+Require Import Coq.Bool.Bool.
+Require Import Coq.Logic.Eqdep.
+Require Import Coq.Logic.Eqdep_dec.
+Require Import Coq.Logic.Decidable.
+Require Import Coq.Program.Equality.
+Require Import Coq.Program.Utils.
+Require Import Lists.ListSet.
+Require Import List.
+Require Import Nat.
+
+Require Util Graph Evaluation Unchanged Disjoint.
+
+Module LoopSplits.
+  Import Util Evaluation.Evaluation Disjoint.Disjoint.
+
+  Lemma lc_loop_split p p0 p0' i0 i0' q1 q2 j1 j2 br' i i' l1 l2 l1' l2' :
+    l1' = nlcons (q1,j1) l1
+    -> l2' = nlcons (q2,j2) l2
+    -> TPath (p0,i0) (p,i) ((p,i) :<: l1')
+    -> TPath (p0',i0') (p,i) ((p,i) :<: l2')
+    -> q1 =/= q2
+    -> i =/= i'
+    -> last_common l1' l2' (br',i')
+    -> exists x', In (br',x') (loop_splits p).
+  Admitted.
+  
+End LoopSplits.
